prove slice::append and progress on array::concat

Lampe/Tests/LenBuiltin.lean
@@ -17,14 +17,67 @@ noir_def std::slice::append<T: Type>(mut self: Slice<T>, other: Slice<T>) -> Sli
   self
 }
 
-def appendEnv : Env := .mk [«std::slice::append»] []
+noir_def std::array::concat<T: Type, N: u32, M: u32>(self: Array<T, N: u32>, array2: Array<T, M: u32>) -> Array<T, (N + M): u32> := {
+  let mut (result: Array<T, (N + M): u32>) = (#_mkRepeatedArray returning Array<T, (N + M): u32>)((#_zeroed returning T)());
+  for i in (0: u32) .. uConst!(N: u32) do {
+    (result[i]: T) = (#_arrayIndex returning T)(self, (#_cast returning u32)(i));
+    #_skip
+  };
+  for i in (0: u32) .. uConst!(M: u32) do {
+    let (i_3606: Unit) = (#_uAdd returning u32)(i, uConst!(N: u32));
+    (result[i_3606]: T) = (#_arrayIndex returning T)(array2, (#_cast returning u32)(i));
+    #_skip
+  };
+  result
+}
 
-set_option Lampe.pp.Expr true
-set_option Lampe.pp.STHoare true
+def thmEnv : Env := .mk [«std::slice::append», «std::array::concat»] []
 
-example : STHoare p appendEnv ⟦⟧ («std::slice::append».call h![T] h![s₁, s₂])
+example (hLen : s₂.length < 2 ^ 32) : STHoare p thmEnv ⟦⟧ («std::slice::append».call h![T] h![s₁, s₂])
     fun v => v = s₁ ++ s₂ := by
   enter_decl
   steps
-  step_as ([self ↦ ⟨Tp.slice T, s₁⟩]) (fun v => v = ())
+  step_as ([self ↦ ⟨Tp.slice T, s₁⟩]) (fun v => ⟦v = ()⟧⋆[self ↦ ⟨Tp.slice T, s₁ ++ s₂⟩])
   · steps
+    subst_vars; assumption
+    loop_inv nat (fun i _ _ => [self ↦ ⟨Tp.slice T, s₁ ++ (s₂.take i)⟩])
+    · simp
+    · congr; simp
+    · intros i hlo hhi
+      steps
+      simp_all
+      subst_vars
+      congr
+      rename_i ha _
+      let ⟨_, h⟩ := ha
+      have : i % 4294967296 = i := by omega
+      simp [this] at h
+      simp [h]
+    steps
+    subst_vars
+    congr
+    simp
+    rw [Nat.mod_eq_of_lt]
+    assumption
+  steps
+  assumption
+
+lemma innercast : (Tp.denote p (Tp.array T (N + M))) = List.Vector (Tp.denote p T) (N.toNat + M.toNat) := by
+  sorry
+
+lemma outercast : («std::array::concat».fn.body (Tp.denote p) h![T, N, M]).outTp = (Tp.array T (N + M)) := by
+  sorry
+
+set_option trace.Lampe.STHoare.Helpers true
+
+example : STHoare p thmEnv ⟦⟧ («std::array::concat».call h![T, N, M] h![arr₁, arr₂])
+    fun v => v = outercast ▸ innercast ▸ (arr₁ ++ arr₂) := by
+  enter_decl
+  steps
+  let x := List.Vector.replicate (N + M).toNat (Tp.zero p T) -- not right, but testing for now
+  loop_inv nat fun i hlo hhi => [result ↦ ⟨Tp.array T (BitVec.add N M), x⟩]
+  · sorry
+  -- apply STHoare.letIn_trivial_intro
+  -- -- let h := @STHoare.loop_inv_intro 32 0 (N + M).toNat p Tp.unit thmEnv
+  -- --   fun i _ _ => [result ↦ ⟨Tp.array T (N + M), x⟩]
+  -- apply STHoare.loop_inv_intro (fun i _ _ => [result ↦ ⟨Tp.array T (N + M), x⟩])
